theories/heap_lang/lib/lock.v
@@ -3,12 +3,18 @@ From iris.heap_lang Require Import proofmode notation.
 From iris.proofmode Require Import tactics.
 Import uPred.
 
-(** * Lock interface *)
-Structure lock Σ `{!heapG Σ} := Lock {
-  (* -- operations -- *)
+(** * Lock operations *)
+Class LockImpl : Set := lock_impl {
   newlock' : val;
   acquire : val;
-  release : val;
+  release : val
+}.
+Arguments newlock' _ : clear implicits.
+Arguments acquire _ : clear implicits.
+Arguments release _ : clear implicits.
+
+(** * Lock interface *)
+Structure lock Σ `{!heapG Σ} {LI : LockImpl} := Lock {
   (* -- predicates -- *)
   (* name is used to associate locked with is_lock *)
   name : Type;
@@ -22,35 +28,33 @@ Structure lock Σ `{!heapG Σ} := Lock {
   (* -- operation specs -- *)
   newlock'_spec p N (R : iProp Σ) :
     heapN ⊥ N →
-    {{{ heap_ctx }}} newlock' #() @ p; ⊤
+    {{{ heap_ctx }}} newlock' LI #() @ p; ⊤
     {{{ lk γ, RET lk;  is_lock N γ lk R ∗ locked γ }}};
   acquire_spec p N γ lk R :
-    {{{ is_lock N γ lk R }}} acquire lk @ p; ⊤ {{{ RET #(); locked γ ∗ R }}};
+    {{{ is_lock N γ lk R }}} acquire LI lk @ p; ⊤ {{{ RET #(); locked γ ∗ R }}};
   release_spec p N γ lk R :
-    {{{ is_lock N γ lk R ∗ locked γ ∗ R }}} release lk @ p; ⊤ {{{ RET #(); True }}}
+    {{{ is_lock N γ lk R ∗ locked γ ∗ R }}} release LI lk @ p; ⊤ {{{ RET #(); True }}}
 }.
 
-Arguments newlock' {_ _} _.
-Arguments acquire {_ _} _.
-Arguments release {_ _} _.
-Arguments is_lock {_ _} _ _ _ _ _.
-Arguments locked {_ _} _ _.
+Arguments name {_ _ _} _.
+Arguments is_lock {_ _ _} _  _ _ _ _.
+Arguments locked {_ _ _} _  _.
 
 Existing Instances is_lock_ne is_lock_persistent locked_timeless.
 
-Instance is_lock_proper Σ `{!heapG Σ} (L: lock Σ) N lk R:
+Instance is_lock_proper Σ `{!heapG Σ, LockImpl} (L: lock Σ) N lk R:
   Proper ((≡) ==> (≡)) (is_lock L N lk R) := ne_proper _.
 
 (** * The [newlock] function *)
-Section newlock.
-  Context `{heapG Σ} (L : lock Σ).
+Definition newlock (LI : LockImpl) : val := λ: <>,
+  let: "lk" := newlock' LI #() in release LI "lk" ;; "lk".
 
-  Definition newlock : val := λ: <>,
-    let: "lk" := newlock' L #() in release L "lk" ;; "lk".
+Section newlock.
+  Context `{heapG Σ, LI : LockImpl} (L : lock Σ).
 
   Lemma newlock_spec p N (R : iProp Σ) :
     heapN ⊥ N →
-    {{{ heap_ctx ∗ R }}} newlock #() @ p; ⊤
+    {{{ heap_ctx ∗ R }}} newlock LI #() @ p; ⊤
     {{{ lk γ, RET lk; is_lock L N γ lk R }}}.
   Proof.
     iIntros (? Φ) "[#Hh Hr] HΦ"; wp_lam.
@@ -63,13 +67,17 @@ Section newlock.
 End newlock.
 
 (** * The [sync_with] and [make_sync] functions *)
-Section sync.
-  Context `{heapG Σ} (L : lock Σ).
+Section sync_code.
+  Context (LI : LockImpl).
 
   Definition sync_with : val := λ: "lk" "f",
-    acquire L "lk" ;; let: "r" := "f" #() in release L "lk" ;; "r".
+    acquire LI "lk" ;; let: "r" := "f" #() in release LI "lk" ;; "r".
   Definition make_sync : val := λ: <>,
-    let: "lk" := newlock L #() in sync_with "lk".
+    let: "lk" := newlock LI #() in sync_with "lk".
+End sync_code.
+
+Section sync_proof.
+  Context `{heapG Σ, LI : LockImpl} (L : lock Σ).
 
   Definition is_sync (sync : val) (R : iProp Σ) : iProp Σ := (
     □ ∀ p e Φ, ⌜Closed [] e⌝ -∗
@@ -84,7 +92,7 @@ Section sync.
   Proof. solve_proper. Qed.
 
   Lemma sync_with_spec p N γ lk (R : iProp Σ) :
-    {{{ is_lock L N γ lk R }}} sync_with lk @ p; ⊤
+    {{{ is_lock L N γ lk R }}} sync_with LI lk @ p; ⊤
     {{{ sync, RET sync; is_sync sync R }}}.
   Proof.
     iIntros (Φ) "#Hlk HΦ". wp_lam.
@@ -98,19 +106,18 @@ Section sync.
 
   Lemma make_sync_spec p N (R : iProp Σ) :
     heapN ⊥ N →
-    {{{ heap_ctx ∗ R }}} make_sync #() @ p; ⊤
+    {{{ heap_ctx ∗ R }}} make_sync LI #() @ p; ⊤
     {{{ sync, RET sync; is_sync sync R }}}.
   Proof.
     iIntros (? Φ) "[#Hh HR] HΦ"; wp_lam.
-    wp_bind (newlock _ _);
-      iApply (newlock_spec _ _ _ R with "[$Hh $HR]"); first done;
-      iNext; iIntros (lk γ) "#Hlk"; wp_let.
+    wp_bind (newlock _ _).
+      iApply (newlock_spec _ _ _ R with "[$Hh $HR]"); first done.
+      iNext. iIntros (lk γ) "#Hlk". wp_let.
     by iApply (sync_with_spec with "[$Hlk] [$HΦ]").
   Qed.
-End sync.
+End sync_proof.
 
 Typeclasses Opaque is_sync.
-Instance: Params (@is_sync) 2.
 
 Instance is_sync_proper Σ `{heapG Σ} sync :
   Proper ((≡) ==> (≡)) (is_sync sync) := ne_proper _.
