theories/tests/lock.v
@@ -1,0 +1,45 @@
+From iris.heap_lang Require Import heap adequacy.
+From iris.heap_lang.lib Require Import lock.
+From iris.heap_lang.lib Require spin_lock.
+From iris.proofmode Require Import tactics.
+From iris.heap_lang Require Import proofmode notation.
+
+(**
+	Ensure we can still apply metatheorems to code using locks.
+*)
+
+Definition ignore_lock (LI : LockImpl) : expr :=
+  let: "lk" := newlock LI #() in
+  #().
+
+Section proof.
+  Context `{heapG Σ, LI : LockImpl} (L : lock Σ).
+
+  Lemma ignore_lock_spec N :
+    heapN ⊥ N →
+    {{{ heap_ctx }}} ignore_lock LI {{{ v, RET v; low v }}}.
+  Proof.
+    iIntros (? Φ) "#Hh HΦ". rewrite/ignore_lock.
+    wp_apply (newlock_spec L _ _ True%I with "[$Hh]"); first done.
+      iIntros (lk γ) "Hlk". wp_let.
+    iApply "HΦ". by simpl_low.
+  Qed.
+End proof.
+
+Section ClosedProof.
+  Import spin_lock.
+
+  Let Σ : gFunctors := #[ heapΣ ; lockΣ ].
+
+  Lemma ignore_lock_safe C t2 σ2 :
+    adv_ctx C →
+    rtc step ([ctx_fill C $ ignore_lock spin], good_state ∅) (t2, σ2) →
+    is_good σ2.
+  Proof.
+    set N : namespace := nroot .@ "ignore_lock".
+    move=>??. eapply (robust_safety Σ); try done.
+    { naive_solver eauto using is_closed_of_val. }
+    iIntros (?) "Hh".
+    iApply (ignore_lock_spec spin_lock N with "Hh"); auto with ndisj.
+  Qed.
+End ClosedProof.
